More module reorganizing

Parser.v
@@ -1,399 +1,356 @@
 Require Import FMaps List MSets Omega String Program.Wf Arith.Wf_nat.
 Require Import Grammar.
+Require Import Lemmas.
 Require Import Tactics.
-Require Import Proofs.Lemmas.
-Require Import ParseTable. 
-Require Import ParseTableGen. (* for fromNtList *)
 Import ListNotations.
 Open Scope string_scope.
 
-Section TripleLT.
-
-  Variables (A B C : Type) (ltA : relation A) (ltB : relation B) (ltC : relation C).
-
-  Inductive triple_lex : A * B * C -> A * B * C -> Prop :=
-  | fst_lt : forall x x' y y' z z', ltA x x' -> triple_lex (x, y, z) (x', y', z')
-  | snd_lt : forall x y y' z z', ltB y y' -> triple_lex (x, y, z) (x, y', z')
-  | thd_lt : forall x y z z', ltC z z' -> triple_lex (x, y, z) (x, y, z').
-
-  Hint Constructors triple_lex.
-
-  Theorem triple_lex_trans :
-    transitive _ ltA -> transitive _ ltB -> transitive _ ltC -> transitive _ triple_lex.
+Module ParserFn (Import G : Grammar.T).
+  Module Import L := LemmasFn G.
+  
+  Definition t_eq_dec  := G.Init.SymTy.t_eq_dec.
+  Definition nt_eq_dec := G.Init.SymTy.nt_eq_dec.
+  
+  Section TripleLT.
+    
+    Variables (A B C : Type) (ltA : relation A) (ltB : relation B) (ltC : relation C).
+    
+    Inductive triple_lex : A * B * C -> A * B * C -> Prop :=
+    | fst_lt : forall x x' y y' z z', ltA x x' -> triple_lex (x, y, z) (x', y', z')
+    | snd_lt : forall x y y' z z', ltB y y' -> triple_lex (x, y, z) (x, y', z')
+    | thd_lt : forall x y z z', ltC z z' -> triple_lex (x, y, z) (x, y, z').
+    
+    Hint Constructors triple_lex.
+    
+    Theorem triple_lex_trans :
+      transitive _ ltA -> transitive _ ltB -> transitive _ ltC -> transitive _ triple_lex.
+    Proof.
+      intros tA tB tC [[x1 y1] z1] [[x2 y2] z2] [[x3 y3] z3] H12 H23.
+      inv H12; inv H23; eauto.
+    Defined.
+    
+    Theorem triple_lex_wf :
+      well_founded ltA -> well_founded ltB -> well_founded ltC -> well_founded triple_lex.
+    Proof.
+      intros wfA wfB wfC [[x y] z].
+      revert y z.
+      induction (wfA x) as [x _ IHx].
+      intros y.
+      induction (wfB y) as [y _ IHy].
+      intros z.
+      induction (wfC z) as [z _ IHz].
+      constructor.
+      intros [[x' y'] z'] H.
+      inv H; eauto.
+    Defined.
+    
+  End TripleLT.
+  
+  Inductive sym_arg  :=
+  | F_arg : symbol -> sym_arg
+  | G_arg : list symbol -> sym_arg.
+  
+  Definition nt_keys (tbl : parse_table) : list nonterminal :=
+    List.map (fun pr => match pr with 
+                        | ((x, _), _) => x
+                        end)
+             (ParseTable.elements tbl).
+  
+  Lemma not_in_list_iff_not_in_fromNtList:
+    forall (x : NtSet.elt) (l : list NtSet.elt),
+      ~ In x l <-> ~ NtSet.In x (fromNtList l).
   Proof.
-    intros tA tB tC [[x1 y1] z1] [[x2 y2] z2] [[x3 y3] z3] H12 H23.
-    inv H12; inv H23; eauto.
+    split; unfold not; intros H1 H2.
+    - apply H1.
+      apply in_list_iff_in_fromNtList; auto.
+    - apply H1.
+      apply in_list_iff_in_fromNtList; auto.
   Defined.
-
-  Theorem triple_lex_wf :
-    well_founded ltA -> well_founded ltB -> well_founded ltC -> well_founded triple_lex.
+  
+  Lemma lt_trans : transitive nat lt.
   Proof.
-    intros wfA wfB wfC [[x y] z].
-    revert y z.
-    induction (wfA x) as [x _ IHx].
-    intros y.
-    induction (wfB y) as [y _ IHy].
-    intros z.
-    induction (wfC z) as [z _ IHz].
-    constructor.
-    intros [[x' y'] z'] H.
-    inv H; eauto.
+    red.
+    apply Nat_as_DT.lt_trans.
   Defined.
-
-End TripleLT.
-
-Section PairLT.
-
-  Variables (A B : Type) (ltA : relation A) (ltB : relation B).
-
-  Inductive pair_lex : A * B  -> A * B  -> Prop :=
-  | pr_fst : forall x x' y y', ltA x x' -> pair_lex (x, y) (x', y')
-  | pr_snd : forall x y y', ltB y y' -> pair_lex (x, y) (x, y').
-
-  Hint Constructors pair_lex.
-
-  Theorem pair_lex_trans :
-    transitive _ ltA -> transitive _ ltB -> transitive _ pair_lex.
+  
+  Lemma pt_lookup_in_nt_keys :
+    forall x la tbl gamma,
+      pt_lookup x la tbl = Some gamma
+      -> In x (nt_keys tbl).
   Proof.
-    intros tA tB [x1 y1] [x2 y2] [x3 y3] H12 H23.
-    inv H12; inv H23; eauto.
+    intros.
+    unfold nt_keys.
+    apply pt_lookup_elements in H.
+    induction (ParseTable.elements tbl).
+    - inv H.
+    - simpl in *.
+      destruct H.
+      + subst; auto.
+      + right; auto.
   Defined.
-
-  Theorem pair_lex_wf :
-    well_founded ltA -> well_founded ltB -> well_founded pair_lex.
+  
+  Definition ptlk_dec x la tbl : Datatypes.sum (pt_lookup x la tbl = None) {gamma | pt_lookup x la tbl = Some gamma}.
+    destruct (pt_lookup x la tbl) eqn:Hlk.
+    - right.
+      econstructor; eauto.
+    - left.
+      auto.
+  Defined.
+  
+  Inductive sa_order : sym_arg -> sym_arg -> Prop := 
+  | f_lt_g : forall sym gamma,
+      sa_order (F_arg sym) (G_arg gamma)
+  | g'_lt_g : forall gamma' gamma,
+      List.length gamma' < List.length gamma
+      -> sa_order (G_arg gamma') (G_arg gamma).
+  
+  Definition meas tbl (word : list terminal) (vis : NtSet.t) (sa : sym_arg) :=
+    (List.length word,
+     NtSet.cardinal (NtSet.diff (fromNtList (nt_keys tbl)) vis),
+     sa).
+  
+  Definition triple_lt : relation (nat * nat * sym_arg) :=
+    triple_lex nat nat sym_arg lt lt sa_order.
+  
+  Lemma sa_order_wf'' :
+    forall sym, Acc sa_order (F_arg sym).
   Proof.
-    intros wfA wfB [x y].
-    revert y.
-    induction (wfA x) as [x _ IHx].
-    intros y.
-    induction (wfB y) as [y _ IHy].
-    constructor.
-    intros [x' y'] H.
-    inv H; eauto.
+    intros.
+    constructor; intros a H.
+    inv H.
   Defined.
-
-End PairLT.
-
-Inductive sym_arg : Set :=
-| F_arg : symbol -> sym_arg
-| G_arg : list symbol -> sym_arg.
-
-Definition nt_keys (tbl : parse_table) : list nonterminal :=
-  List.map (fun pr => match pr with 
-                      | ((x, _), _) => x
-                      end)
-           (ParseTable.elements tbl).
-
-Lemma not_in_list_iff_not_in_fromNtList:
-  forall (x : NtSet.elt) (l : list NtSet.elt),
-    ~ In x l <-> ~ NtSet.In x (fromNtList l).
-Proof.
-  split; unfold not; intros H1 H2.
-  - apply H1.
-    apply in_list_iff_in_fromNtList; auto.
-  - apply H1.
-    apply in_list_iff_in_fromNtList; auto.
-Defined.
-
-Lemma lt_trans : transitive nat lt.
-Proof.
-  red.
-  apply Nat_as_DT.lt_trans.
-Defined.
-
-Lemma pt_lookup_in_nt_keys :
-  forall x la tbl gamma,
-    pt_lookup x la tbl = Some gamma
-    -> In x (nt_keys tbl).
-Proof.
-  intros.
-  unfold nt_keys.
-  apply pt_lookup_elements in H.
-  induction (ParseTable.elements tbl).
-  - inv H.
-  - simpl in *.
-    destruct H.
-    + subst; auto.
-    + right; auto.
-Defined.
-        
-Definition ptlk_dec x la tbl : sum (pt_lookup x la tbl = None) {gamma | pt_lookup x la tbl = Some gamma}.
-  destruct (pt_lookup x la tbl) eqn:Hlk.
-  - right.
-    econstructor; eauto.
-  - left.
-    auto.
-Defined.
-
-Definition X := 0.
-Definition Y := 1.
-Definition Z := 2.
-
-Definition yy_grammar :=
-  {|
-     start := X
-   ; productions := [(X, [NT Y; NT Y; T "a"]);
-                     (Y, [])]
-  |}.
-
-Definition a_generator :=
-  {|
-     start := X
-   ; productions := [(X, [T "a"; NT X]);
-                     (X, [])]
-  |}.
-
-Definition lr_table :=
-  ParseTable.add (X, LA "a") [NT Y; NT Z]
-                 (ParseTable.add (Y, LA "a") []
-                                 (ParseTable.add (Z, LA "a") [NT X]
-                                                 (ParseTable.empty (list symbol)))).
-
-Inductive sa_order : sym_arg -> sym_arg -> Prop := 
-| f_lt_g : forall sym gamma,
-    sa_order (F_arg sym) (G_arg gamma)
-| g'_lt_g : forall gamma' gamma,
-    List.length gamma' < List.length gamma
-    -> sa_order (G_arg gamma') (G_arg gamma).
-
-Definition meas tbl (word : list string) (vis : NtSet.t) (sa : sym_arg) :=
-  (List.length word,
-   NtSet.cardinal (NtSet.diff (fromNtList (nt_keys tbl))                                  vis),
-   sa).
-
-Definition triple_lt : relation (nat * nat * sym_arg) :=
-  triple_lex nat nat sym_arg lt lt sa_order.
-
-Lemma sa_order_wf'' :
-  forall sym, Acc sa_order (F_arg sym).
-Proof.
-  intros.
-  constructor; intros a H.
-  inv H.
-Defined.
-
-Lemma sa_order_wf' :
-  forall n gamma,
-    List.length gamma < n
-    -> Acc sa_order (G_arg gamma).
-Proof.
-  induction n; intros gamma H; simpl in *.
-  - inv H.
-  - constructor; intros a Ha.
-    inv Ha; simpl in *.
-    + apply sa_order_wf''.
-    + apply IHn; omega.
-Defined.
-
-Theorem sa_order_wf : well_founded sa_order.
-Proof.
-  red; intros a; destruct a.
-  - apply sa_order_wf''.
-  - eapply sa_order_wf'; eauto.
-Defined.
-
-Theorem triple_lt_wf : well_founded triple_lt.
-  apply triple_lex_wf; try apply lt_wf.
-  apply sa_order_wf.
-Defined.
-
-Lemma hole1 :
-  forall tbl input vis sa sa' x gamma,
-    Acc triple_lt (meas tbl input vis sa)
-    -> pt_lookup x (peek input) tbl = Some gamma
-    -> ~ NtSet.In x vis
-    -> Acc triple_lt (meas tbl input (NtSet.add x vis) sa').
-Proof.
-  intros.
-  eapply Acc_inv; eauto.
-  unfold meas.
-  apply snd_lt; simpl.
-  apply NP.subset_cardinal_lt with (x := x); try ND.fsetdec.
-  apply in_A_not_in_B_in_diff; auto.
-  apply in_list_iff_in_fromNtList.
-  eapply pt_lookup_in_nt_keys; eauto.
-Defined.
-
-Lemma hole2 :
-  forall tbl input vis gamma sym,
-    Acc triple_lt (meas tbl input vis (G_arg gamma))
-    -> Acc triple_lt (meas tbl input vis (F_arg sym)).
-Proof.
-  intros.
-  eapply Acc_inv; eauto.
-  apply thd_lt; constructor.
-Defined.
-
-Lemma hole3 :
-  forall tbl input input' vis vis' sa sa',
-    Acc triple_lt (meas tbl input vis sa)
-    -> List.length input' < List.length input
-    -> Acc triple_lt (meas tbl input' vis' sa').
-Proof.
-  intros.
-  eapply Acc_inv; eauto.
-  apply fst_lt; auto.
-Defined.
-
-Lemma hole4 :
-  forall tbl input vis gamma sym gamma',
-    Acc triple_lt (meas tbl input vis (G_arg gamma))
-    -> gamma = sym :: gamma'
-    -> Acc triple_lt (meas tbl input vis (G_arg gamma')).
-Proof.
-  intros.
-  eapply Acc_inv; eauto.
-  apply thd_lt; subst.
-  constructor; auto.
-Defined.
-
-Ltac step_h := match goal with
-               | H : context[match ?x with | _ => _ end] |- _ => destruct x
-              end.
-
-Ltac step_h_eq s := let Heq := fresh s in
-                    match goal with
-                    | H : context[match ?x with | _ => _ end] |- _ =>
-                      destruct x eqn:Heq
-                    end.
-
-Ltac step_g := match goal with
-               | |- context[match ?x with | _ => _ end] => destruct x
-               end.
-
-Ltac step_g_eq s := let Heq := fresh s in
-                    match goal with
-                    | |- context[match ?x with | _ => _ end] => destruct x eqn:Heq
-                    end.
-
-Ltac step := simpl in *; (first [step_h | step_g]); auto.
-Ltac step_eq s := simpl in *; (first [step_h_eq s | step_g_eq s]); auto.
-Ltac cr := repeat step.
-Ltac cr_eq s := repeat (step_eq s).
-Ltac tc := try congruence.
-
-Open Scope list_scope.
-
-Lemma l_ident_eq_nil :
-  forall A (xs ys : list A), xs ++ ys = ys -> xs = [].
-Proof.
-  intros.
-  rewrite <- app_nil_l in H.
-  apply app_inv_tail in H; auto.
-Qed.
-
-Inductive parse_failure : Type :=
-| Reject   : string -> list string -> parse_failure
-| LeftRec  : nonterminal -> NtSet.t -> list string -> parse_failure.
-
-Definition mem_dec (x : nonterminal) (s : NtSet.t) : {NtSet.In x s} + {~ NtSet.In x s}.
-  destruct (NtSet.mem x s) eqn:Hm.
-  - left.
-    apply NtSet.mem_spec; auto.
-  - right.
-    unfold not; intros H.
-    apply NtSet.mem_spec in H.
-    congruence.
-Defined.
-
-Definition length_lt_eq A (xs ys : list A) :=
-  {List.length xs < List.length ys} + {xs = ys}.
-
-Lemma length_lt_eq_cons : forall A xs (x : A) xs',
-    xs = x :: xs'
-    -> length_lt_eq A xs' xs.
-Proof.
-  intros; simpl; red; subst; auto.
-Defined.
-
-Lemma length_lt_eq_refl : forall A (xs : list A),
-    length_lt_eq A xs xs.
-Proof.
-  intros; simpl; red; auto.
-Defined.
-
-Lemma length_lt_eq_trans :
-  forall A (xs ys zs : list A),
-    length_lt_eq A xs ys
-    -> length_lt_eq A ys zs
-    -> length_lt_eq A xs zs.
-Proof.
-  intros A xs ys zs H H'; unfold length_lt_eq in *;
-    destruct H; destruct H'; subst; auto.
-  left; omega.
-Defined.
-
-Fixpoint parse_nf
-         (tbl : parse_table)
-         (sym : symbol)
-         (input : list string)
-         (vis : NtSet.t)
-         (a : Acc triple_lt (meas tbl input vis (F_arg sym)))
-         {struct a}
-  : sum parse_failure (tree * {input' & length_lt_eq _ input' input}) :=
-  match sym with
-  | T a =>
-    match input as i return input = i -> _ with
-    | nil =>
-      fun _ => inl (Reject "input exhausted" input)
-    | token :: input' => 
-      fun Hin => 
-        if string_dec a token then
-          inr (Leaf a, existT _ input' (length_lt_eq_cons _ _ _ _ Hin))
-        else
-          inl (Reject "token mismatch" input)
-    end eq_refl
-  | NT x =>
-    match ptlk_dec x (peek input) tbl with
-    | inl _ => inl (Reject "lookup failure" input)
-    | inr (exist _ gamma Hlk) =>
-      match mem_dec x vis with
-      | left _ => inl (LeftRec x vis input)
-      | right Hnin =>
-        match parseForest_nf tbl gamma input (NtSet.add x vis) (hole1 _ _ _ _ _ _ _ a Hlk Hnin) with
-        | inl pfail => inl pfail
-        | inr (sts, existT _ input' Hle) =>
-          inr (Node x sts, existT _ input' Hle)
+  
+  Lemma sa_order_wf' :
+    forall n gamma,
+      List.length gamma < n
+      -> Acc sa_order (G_arg gamma).
+  Proof.
+    induction n; intros gamma H; simpl in *.
+    - inv H.
+    - constructor; intros a Ha.
+      inv Ha; simpl in *.
+      + apply sa_order_wf''.
+      + apply IHn; omega.
+  Defined.
+  
+  Theorem sa_order_wf : well_founded sa_order.
+  Proof.
+    red; intros a; destruct a.
+    - apply sa_order_wf''.
+    - eapply sa_order_wf'; eauto.
+  Defined.
+  
+  Theorem triple_lt_wf : well_founded triple_lt.
+    apply triple_lex_wf; try apply lt_wf.
+    apply sa_order_wf.
+  Defined.
+  
+  Lemma hole1 :
+    forall tbl input vis sa sa' x gamma,
+      Acc triple_lt (meas tbl input vis sa)
+      -> pt_lookup x (peek input) tbl = Some gamma
+      -> ~ NtSet.In x vis
+      -> Acc triple_lt (meas tbl input (NtSet.add x vis) sa').
+  Proof.
+    intros.
+    eapply Acc_inv; eauto.
+    unfold meas.
+    apply snd_lt; simpl.
+    apply NP.subset_cardinal_lt with (x := x); try ND.fsetdec.
+    apply in_A_not_in_B_in_diff; auto.
+    apply in_list_iff_in_fromNtList.
+    eapply pt_lookup_in_nt_keys; eauto.
+  Defined.
+  
+  Lemma hole2 :
+    forall tbl input vis gamma sym,
+      Acc triple_lt (meas tbl input vis (G_arg gamma))
+      -> Acc triple_lt (meas tbl input vis (F_arg sym)).
+  Proof.
+    intros.
+    eapply Acc_inv; eauto.
+    apply thd_lt; constructor.
+  Defined.
+  
+  Lemma hole3 :
+    forall tbl input input' vis vis' sa sa',
+      Acc triple_lt (meas tbl input vis sa)
+      -> List.length input' < List.length input
+      -> Acc triple_lt (meas tbl input' vis' sa').
+  Proof.
+    intros.
+    eapply Acc_inv; eauto.
+    apply fst_lt; auto.
+  Defined.
+  
+  Lemma hole4 :
+    forall tbl input vis gamma sym gamma',
+      Acc triple_lt (meas tbl input vis (G_arg gamma))
+      -> gamma = sym :: gamma'
+      -> Acc triple_lt (meas tbl input vis (G_arg gamma')).
+  Proof.
+    intros.
+    eapply Acc_inv; eauto.
+    apply thd_lt; subst.
+    constructor; auto.
+  Defined.
+  
+  Ltac step_h := match goal with
+                 | H : context[match ?x with | _ => _ end] |- _ => destruct x
+                 end.
+  
+  Ltac step_h_eq s := let Heq := fresh s in
+                      match goal with
+                      | H : context[match ?x with | _ => _ end] |- _ =>
+                        destruct x eqn:Heq
+                      end.
+  
+  Ltac step_g := match goal with
+                 | |- context[match ?x with | _ => _ end] => destruct x
+                 end.
+  
+  Ltac step_g_eq s := let Heq := fresh s in
+                      match goal with
+                      | |- context[match ?x with | _ => _ end] => destruct x eqn:Heq
+                      end.
+  
+  Ltac step := simpl in *; (first [step_h | step_g]); auto.
+  Ltac step_eq s := simpl in *; (first [step_h_eq s | step_g_eq s]); auto.
+  Ltac cr := repeat step.
+  Ltac cr_eq s := repeat (step_eq s).
+  Ltac tc := try congruence.
+  
+  Open Scope list_scope.
+  
+  Lemma l_ident_eq_nil :
+    forall A (xs ys : list A), xs ++ ys = ys -> xs = [].
+  Proof.
+    intros.
+    rewrite <- app_nil_l in H.
+    apply app_inv_tail in H; auto.
+  Qed.
+  
+  Inductive parse_failure : Type :=
+  | Reject   : string -> list terminal -> parse_failure
+  | LeftRec  : nonterminal -> NtSet.t -> list terminal -> parse_failure.
+  
+  Definition mem_dec (x : nonterminal) (s : NtSet.t) : {NtSet.In x s} + {~ NtSet.In x s}.
+    destruct (NtSet.mem x s) eqn:Hm.
+    - left.
+      apply NtSet.mem_spec; auto.
+    - right.
+      unfold not; intros H.
+      apply NtSet.mem_spec in H.
+      congruence.
+  Defined.
+  
+  Definition length_lt_eq A (xs ys : list A) :=
+    {List.length xs < List.length ys} + {xs = ys}.
+  
+  Lemma length_lt_eq_cons : forall A xs (x : A) xs',
+      xs = x :: xs'
+      -> length_lt_eq A xs' xs.
+  Proof.
+    intros; simpl; red; subst; auto.
+  Defined.
+  
+  Lemma length_lt_eq_refl : forall A (xs : list A),
+      length_lt_eq A xs xs.
+  Proof.
+    intros; simpl; red; auto.
+  Defined.
+  
+  Lemma length_lt_eq_trans :
+    forall A (xs ys zs : list A),
+      length_lt_eq A xs ys
+      -> length_lt_eq A ys zs
+      -> length_lt_eq A xs zs.
+  Proof.
+    intros A xs ys zs H H'; unfold length_lt_eq in *;
+      destruct H; destruct H'; subst; auto.
+    left; omega.
+  Defined.
+  
+  Fixpoint parse_nf
+           (tbl : parse_table)
+           (sym : symbol)
+           (input : list terminal)
+           (vis : NtSet.t)
+           (a : Acc triple_lt (meas tbl input vis (F_arg sym)))
+           {struct a}
+    : Datatypes.sum parse_failure (tree * {input' & length_lt_eq _ input' input}) :=
+    match sym with
+    | T a =>
+      match input as i return input = i -> _ with
+      | nil =>
+        fun _ => inl (Reject "input exhausted" input)
+      | token :: input' => 
+        fun Hin => 
+          if t_eq_dec a token then
+            inr (Leaf a, existT _ input' (length_lt_eq_cons _ _ _ _ Hin))
+          else
+            inl (Reject "token mismatch" input)
+      end eq_refl
+    | NT x =>
+      match ptlk_dec x (peek input) tbl with
+      | inl _ => inl (Reject "lookup failure" input)
+      | inr (exist _ gamma Hlk) =>
+        match mem_dec x vis with
+        | left _ => inl (LeftRec x vis input)
+        | right Hnin =>
+          match parseForest_nf tbl gamma input (NtSet.add x vis)
+                               (hole1 _ _ _ _ _ _ _ a Hlk Hnin)
+          with
+          | inl pfail => inl pfail
+          | inr (sts, existT _ input' Hle) =>
+            inr (Node x sts, existT _ input' Hle)
+          end
         end
       end
     end
-  end
-with parseForest_nf (tbl : parse_table)
-     (gamma : list symbol)
-     (input : list string)
-     (vis : NtSet.t)
-     (a : Acc triple_lt (meas tbl input vis (G_arg gamma)))
-     {struct a}
-     : sum parse_failure (list tree * {input' & length_lt_eq _ input' input}) :=
-    match gamma as g return gamma = g -> _  with
-    | nil => fun _ => inr (nil, existT (fun input' => length_lt_eq string input' input) input
-                                       (length_lt_eq_refl _ _))
-    | sym :: gamma' => fun Hg => 
-                         match parse_nf tbl sym input vis (hole2 _ _ _ _ _ a) with
-                         | inl pfail => inl pfail
-                         | inr (lSib, existT _ input' Hle) =>
-                           match Hle with
-                           | left Hlt =>
-                             match parseForest_nf tbl gamma' input' NtSet.empty (hole3 _ _ _ _ _ _ _ a Hlt) with
-                             | inl pfail => inl pfail
-                             | inr (rSibs, existT _ input'' Hle'') =>
-                               inr (lSib :: rSibs, existT _ input'' (length_lt_eq_trans _ _ _ _ Hle'' Hle))
-                             end
-                           | right Heq =>
-                             match parseForest_nf tbl gamma' input vis (hole4 _ _ _ _ _ _ a Hg) with
-                             | inl pfail => inl pfail
-                             | inr (rSibs, existT _ input'' Hle'') =>
-                               inr (lSib :: rSibs, existT _ input'' Hle'')
-                             end
-                           end
-                         end
-    end eq_refl.
+  with parseForest_nf (tbl : parse_table)
+                      (gamma : list symbol)
+                      (input : list terminal)
+                      (vis : NtSet.t)
+                      (a : Acc triple_lt (meas tbl input vis (G_arg gamma)))
+                      {struct a}
+       : Datatypes.sum parse_failure (list tree * {input' & length_lt_eq _ input' input}) :=
+         match gamma as g return gamma = g -> _  with
+         | nil => fun _ => inr (nil, existT (fun input' => length_lt_eq terminal input' input)
+                                            input
+                                            (length_lt_eq_refl _ _))
+         | sym :: gamma' => fun Hg => 
+                              match parse_nf tbl sym input vis (hole2 _ _ _ _ _ a) with
+                              | inl pfail => inl pfail
+                              | inr (lSib, existT _ input' Hle) =>
+                                match Hle with
+                                | left Hlt =>
+                                  match parseForest_nf tbl gamma' input' NtSet.empty
+                                                       (hole3 _ _ _ _ _ _ _ a Hlt)
+                                  with
+                                  | inl pfail => inl pfail
+                                  | inr (rSibs, existT _ input'' Hle'') =>
+                                    inr (lSib :: rSibs, existT _ input'' (length_lt_eq_trans _ _ _ _ Hle'' Hle))
+                                  end
+                                | right Heq =>
+                                  match parseForest_nf tbl gamma' input vis
+                                                       (hole4 _ _ _ _ _ _ a Hg)
+                                  with
+                                  | inl pfail => inl pfail
+                                  | inr (rSibs, existT _ input'' Hle'') =>
+                                    inr (lSib :: rSibs, existT _ input'' Hle'')
+                                  end
+                                end
+                              end
+         end eq_refl.
 
-Definition sa_size (sa : sym_arg) : nat :=
-  match sa with
-  | F_arg _ => 0
-  | G_arg gamma => 1 + List.length gamma
-  end.
-
-Definition parse_wrapper tbl sym input :=
-  parse_nf tbl sym input NtSet.empty (triple_lt_wf (meas tbl input NtSet.empty (F_arg sym))).
+  Definition sa_size (sa : sym_arg) : nat :=
+    match sa with
+    | F_arg _ => 0
+    | G_arg gamma => 1 + List.length gamma
+    end.
+  
+  Definition parse_wrapper tbl sym input :=
+    parse_nf tbl sym input NtSet.empty (triple_lt_wf (meas tbl input NtSet.empty (F_arg sym))).
+  
+End ParserFn.
