Lemmas.v
@@ -81,5 +81,286 @@ Module LemmasFn (Import G : Grammar.T).
     rewrite H0. rewrite in_app_iff.
     right. apply in_eq.
   Qed.
+
+  Lemma pt_find_in :
+  forall k A (v : A) m,
+    ParseTable.find k m = Some v
+    -> ParseTable.In k m.
+Proof.
+  intros.
+  rewrite ParseTableFacts.in_find_iff.
+  rewrite H; congruence.
+Qed.
+
+(*
+Lemma lookaheadmap_find_in : forall k vT (v : vT) m,
+    LaMap.find k m = Some v ->
+    LaMap.In k m.
+Proof.
+  intros. rewrite LaMapFacts.in_find_iff. rewrite H.
+  unfold not. intro Hcontra. inv Hcontra.
+Qed.
+*)
+Lemma pt_lookup_in :
+  forall x la tbl gamma,
+    pt_lookup x la tbl = Some gamma
+    -> ParseTable.In (x, la) tbl.
+Proof.
+  intros x la tbl gamma Hlkp.
+  unfold pt_lookup in Hlkp.
+  apply ParseTableFacts.in_find_iff; congruence.
+Qed.
+
+Lemma eof_first_sym :
+  forall g la sym,
+    first_sym g la sym
+    -> la = EOF
+    -> False.
+Proof.
+  induction 1; intros; auto.
+  inv H.
+Qed.
+
+Lemma eof_first_gamma :
+  forall g la gamma,
+    first_gamma g la gamma
+    -> la = EOF
+    -> False.
+Proof.
+  intros.
+  inv H.
+  eapply eof_first_sym; eauto.
+Qed.
+
+Lemma nullable_middle_sym :
+  forall g xs ys sym,
+    nullable_gamma g (xs ++ sym :: ys)
+    -> nullable_sym g sym.
+Proof.
+  induction xs; intros.
+  - simpl in H.
+    inv H.
+    auto.
+  - eapply IHxs.
+    inv H.
+    eauto.
+Qed.
+
+Lemma gamma_with_terminal_not_nullable :
+  forall g gpre y gsuf,
+    ~ nullable_gamma g (gpre ++ T y :: gsuf).
+Proof.
+  unfold not.
+  induction gpre as [| sym syms]; intros y gsuf Hnu; simpl in *.
+  - inv Hnu.
+    inv H1.
+  - destruct sym.
+    + inv Hnu.
+      inv H1.
+    + inv Hnu.
+      eapply IHsyms; eauto.
+Qed.
+
+Lemma nullable_split :
+  forall g xs ys,
+    nullable_gamma g (xs ++ ys)
+    -> nullable_gamma g ys.
+Proof.
+  induction xs; intros.
+  - auto.
+  - inv H.
+    eapply IHxs; eauto.
+Qed.
+
+(* New version, without mutual induction *)
+Lemma no_first_follow_conflicts :
+  forall tbl g,
+    parse_table_correct tbl g
+    -> forall la sym,
+      first_sym g la sym
+      -> nullable_sym g sym
+      -> follow_sym g la sym
+      -> False.
+Proof.
+  intros tbl g Htbl la sym Hfi.
+  induction Hfi; intros.
+  - inv H.
+  - inv H1.
+    assert (ys = gpre ++ s :: gsuf).
+    { destruct Htbl as [Hmin Hcom].
+      assert (Hlk : lookahead_for la x (gpre ++ s :: gsuf) g).
+      { unfold lookahead_for; auto. }
+      assert (Hlk' : lookahead_for la x ys g).
+      { unfold lookahead_for; auto. }
+      unfold pt_complete in Hcom.
+      apply Hcom in Hlk; auto.
+      apply Hcom in Hlk'; auto.
+      congruence. }
+    subst.
+    eapply IHHfi.
+    + apply nullable_middle_sym in H5; auto.
+    + destruct s.
+      * apply gamma_with_terminal_not_nullable in H5; inv H5.
+      * eapply FollowLeft; eauto.
+        assert (NT n :: gsuf = [NT n] ++ gsuf) by auto.
+        rewrite H1 in H5.
+        rewrite app_assoc in H5.
+        apply nullable_split in H5.
+        auto.
+Qed.
+
+Lemma sym_derives_nil_nullable :
+  forall g sym wpre f wsuf,
+    (@sym_derives_prefix g) sym wpre f wsuf
+    -> wpre = nil
+    -> nullable_sym g sym.
+Proof.
+  intros g sym wpre f wsuf Hder.
+  induction Hder using sdp_mutual_ind with
+      (P := fun sym wpre tr wsuf
+                (pf : sym_derives_prefix sym wpre tr wsuf) =>
+              wpre = nil
+              -> nullable_sym g sym)
+      (P0 := fun gamma wpre f wsuf
+                 (pf : gamma_derives_prefix gamma wpre f wsuf)
+             =>
+               wpre = nil
+               -> nullable_gamma g gamma); intros; subst.
+  - inv H.
+  - simpl in *.
+    econstructor; eauto.
+  - constructor.
+  - apply app_eq_nil in H; destruct H; subst.
+    destruct IHHder; auto.
+    constructor; auto.
+    econstructor; eauto.
+Qed.
+
+Lemma gamma_derives_cons_first_gamma :
+  forall g gamma word f rem,
+    (@gamma_derives_prefix g) gamma word f rem
+    -> forall tok toks,
+      word = tok :: toks
+      -> first_gamma g (LA tok) gamma.
+Proof.
+  intros g gamma word f rem Hder.
+  induction Hder using gdp_mutual_ind with
+      (P := fun sym word tr rem
+                (pf : sym_derives_prefix sym word tr rem) =>
+              forall tok toks,
+                word = tok :: toks
+                -> first_sym g (LA tok) sym)
+      (P0 := fun gamma word f rem
+                 (pf : gamma_derives_prefix gamma word f rem)
+             =>
+               forall tok toks,
+                 word = tok :: toks
+                 -> first_gamma g (LA tok) gamma); intros; subst.
+  - inv H; constructor.
+  - simpl in *.
+    specialize (IHHder tok toks).
+    destruct IHHder; auto.
+    econstructor; eauto.
+  - inv H.
+  - destruct hdRoot.
+    + inv s.
+      inv H.
+      eapply FirstGamma with (gpre := nil); constructor.
+    + destruct wpre as [| ptok ptoks]; simpl in *.
+      * subst.
+        specialize (IHHder0 tok toks).
+        destruct IHHder0; auto.
+        eapply FirstGamma with (gpre := NT n :: gpre).
+        -- constructor; auto.
+           apply sym_derives_nil_nullable in s; auto.
+        -- auto.
+      * inv H.
+        eapply FirstGamma with (gpre := nil).
+        -- constructor.
+        -- eapply IHHder; eauto.
+Qed.
+
+Lemma tbl_entry_is_lookahead :
+  forall tbl g x la gamma,
+    parse_table_correct tbl g
+    -> pt_lookup x la tbl = Some gamma
+    -> lookahead_for la x gamma g.
+Proof.
+  intros tbl g x la gamma Htbl Hlkp.
+  destruct Htbl as [Hsou Hcom].
+  unfold pt_sound in Hsou.
+  apply Hsou; auto.
+Qed.
+
+Lemma first_gamma_first_sym :
+  forall g x la gamma,
+    In (x, gamma) g.(prods)
+    -> first_gamma g la gamma
+    -> first_sym g la (NT x).
+Proof.
+  intros g x la gamma Hin Hfg.
+  inv Hfg.
+  econstructor; eauto.
+Qed.
+
+Lemma in_A_not_in_B_in_diff :
+  forall elt a b,
+    NtSet.In elt a
+    -> ~ NtSet.In elt b
+    -> NtSet.In elt (NtSet.diff a b).
+Proof.
+  ND.fsetdec.
+Defined.
+
+Lemma in_list_iff_in_fromNtList :
+  forall x l, In x l <-> NtSet.In x (fromNtList l).
+Proof.
+  split; intros; induction l; simpl in *.
+  - inv H.
+  - destruct H; subst; auto.
+    + ND.fsetdec.
+    + apply IHl in H; ND.fsetdec.
+  - ND.fsetdec.
+  - destruct (NtSetFacts.eq_dec x a); subst; auto.
+    right. apply IHl. ND.fsetdec.
+Defined.
+
+Lemma pt_lookup_elements' :
+  forall (k : ParseTable.key) (gamma : list symbol) (l : list (ParseTable.key * list symbol)),
+    findA (ParseTableFacts.eqb k) l = Some gamma
+    -> In (k, gamma) l.
+Proof.
+  intros.
+  induction l.
+  - inv H.
+  - simpl in *.
+    destruct a as (k', gamma').
+    destruct (ParseTableFacts.eqb k k') eqn:Heq.
+    + inv H.
+      unfold ParseTableFacts.eqb in *.
+      destruct (ParseTableFacts.eq_dec k k').
+      * subst; auto.
+      * inv Heq.
+    + right; auto.
+Defined.
+      
+Lemma pt_lookup_elements :
+  forall x la tbl gamma,
+    pt_lookup x la tbl = Some gamma
+    -> In ((x, la), gamma) (ParseTable.elements tbl).
+Proof.
+  intros.
+  unfold pt_lookup in *.
+  rewrite ParseTableFacts.elements_o in H.
+  apply pt_lookup_elements'; auto.
+Defined.
+
+  Lemma cons_app_singleton :
+    forall A (x : A) (ys : list A),
+      x :: ys = [x] ++ ys.
+  Proof.
+    auto.
+  Defined.
   
 End LemmasFn.
+
