Main.v
@@ -1,0 +1,81 @@
+Require Import Grammar.
+Require Import mkParseTable_correct.
+Require Import Parser_sound.
+
+Module Main (Import G : Grammar.T).
+
+  Module Import GeneratorProofs := GeneratorProofsFn G.
+  Module Import ParserSoundness := ParserSoundnessFn G.
+
+  Definition parseTableOf (g : grammar) : option parse_table :=
+    let nu := mkNullableSet g in
+    let nu_pf := (mkNullableSet_correct g) in
+    let fi := mkFirstMap g nu in
+    let fi_pf := (mkFirstMap_correct g nu nu_pf) in
+    let fo := mkFollowMap g nu fi fi_pf in
+    let es := mkEntries nu fi fo g in
+    mkParseTable es.
+
+  Theorem parseTableOf_sound : 
+    forall (g : grammar) (tbl : parse_table), 
+      parseTableOf g = Some tbl
+      -> parse_table_correct tbl g.
+  Proof.
+    intros g tbl Hf.
+    eapply mkParseTable_sound; eauto.
+    eapply mkEntries_correct; eauto.
+    - apply mkNullableSet_correct; auto.
+    - apply mkFirstMap_correct.
+      apply mkNullableSet_correct; auto.
+    - apply mkFollowMap_correct; auto.
+      apply mkNullableSet_correct; auto.
+  Qed.
+
+  Theorem parseTableOf_complete :
+    forall (g : grammar) (tbl : parse_table),
+      parse_table_correct tbl g 
+      -> exists (tbl' : parse_table),
+        ParseTable.Equal tbl tbl' /\ parseTableOf g = Some tbl'.
+  Proof.
+    intros g tbl Hpt.
+    eapply mkParseTable_complete; eauto.
+    eapply mkEntries_correct; eauto.
+    - apply mkNullableSet_correct; auto.
+    - apply mkFirstMap_correct.
+      apply mkNullableSet_correct; auto.
+    - apply mkFollowMap_correct; auto.
+      apply mkNullableSet_correct; auto.
+  Qed.
+  
+  Definition parse (tbl : parse_table)
+             (sym : symbol)
+             (input : list terminal) :
+    Datatypes.sum parse_failure (tree * list terminal) :=
+    match parse_nf tbl sym input NtSet.empty
+                   (triple_lt_wf (meas tbl input NtSet.empty (F_arg sym)))
+    with
+    | inl failure => inl failure
+    | inr (tr, existT _ input' Hle) => inr (tr, input')
+    end.
+
+  Theorem parser_sound :
+    forall (g   : grammar)
+           (tbl : parse_table)
+           (sym : symbol)
+           (word rem : list terminal)
+           (tr : tree),
+      parse_table_correct tbl g
+      -> parse tbl sym (word ++ rem) = inr (tr, rem)
+      -> (@sym_derives_prefix g) sym word tr rem.
+  Proof.
+    intros.
+    unfold parse in *.
+    destruct (parse_nf tbl sym (word ++ rem) NtSet.empty (triple_lt_wf (meas tbl (word ++ rem) NtSet.empty (F_arg sym)))) eqn:Hp.
+    - tc.
+    - destruct p.
+      destruct s.
+      inversion H0; subst.
+      eapply parse_sound; eauto.  
+Qed.
+
+End Main.
