Proofs/mkNullableSet_correct.v
@@ -1,0 +1,321 @@
+Require Import MSets.
+Require Import Wf_nat.
+
+Require Import Generator.
+Require Import Grammar.
+Require Import Tactics.
+
+Import ListNotations.
+
+Module NullableProofsFn (Import G : Grammar.T).
+
+  Module Export Gen := GeneratorFn G.
+
+  Lemma mkNullableSet'_eq_body :
+    forall (ps : list production)
+           (nu : NtSet.t),
+      mkNullableSet' ps nu =
+      let nu' := nullablePass ps nu in
+      if NtSet.eq_dec nu nu' then
+        nu
+      else
+        mkNullableSet' ps nu'.
+  Proof.
+    intros ps nu.
+    unfold mkNullableSet'.
+    unfold mkNullableSet'_func.
+    rewrite Wf.fix_sub_eq; auto.
+    intros.
+    match goal with
+    | |- context[NtSet.eq_dec ?a ?b] => destruct (NtSet.eq_dec a b)
+    end; auto.
+  Qed.
+  
+  Lemma nu_sound_nullableGamma_sound :
+    forall (g     : grammar)
+           (nu    : NtSet.t)
+           (gamma : list symbol),
+      nullable_set_sound nu g
+      -> nullableGamma gamma nu = true
+      -> nullable_gamma g gamma.
+  Proof.
+    intros g nu gamma Hsou Hng.
+    induction gamma as [| sym syms]; auto.
+    destruct sym as [y | x].
+    - inv Hng.
+    - simpl in *.
+      destruct (NtSet.mem x nu) eqn:Hmem.
+      + rewrite NtSet.mem_spec in Hmem.
+        apply Hsou in Hmem.
+        econstructor; eauto.
+      + inv Hng.
+  Qed.
+  
+  Lemma cons_app_singleton :
+    forall A (x : A) (ys : list A),
+      x :: ys = [x] ++ ys.
+  Proof.
+    auto.
+  Qed.
+  
+  Lemma in_app_cons :
+    forall A (x : A) (pre suf : list A),
+      In x (pre ++ x :: suf).
+  Proof.
+    intros A x pre suf.
+    induction pre; simpl; auto.
+  Qed.
+  
+  Lemma nullablePass_preserves_soundness' :
+    forall (g  : grammar)
+           (nu : NtSet.t),
+      nullable_set_sound nu g
+      -> forall suf pre : list production,
+        pre ++ suf = g.(prods)
+        -> nullable_set_sound (nullablePass suf nu) g.
+  Proof. 
+    intros g nu Hsou suf.
+    induction suf as [| (x, gamma) suf]; intros pre Happ; simpl; auto.
+    pose proof Happ as Happ'.
+    rewrite cons_app_singleton in Happ.
+    rewrite app_assoc in Happ.
+    apply IHsuf in Happ.
+    destruct (nullableGamma gamma (nullablePass suf nu)) eqn:Hng; auto.
+    unfold nullable_set_sound.
+    intros x' Hin.
+    destruct (NtSetFacts.eq_dec x x'); subst.
+    - econstructor.
+      + rewrite <- Happ'.
+        apply in_app_cons.
+      + eapply nu_sound_nullableGamma_sound; eauto.
+    - apply NtSetFacts.add_3 in Hin; auto.
+  Qed.
+  
+  Lemma nullablePass_preserves_soundness :
+    forall (g  : grammar)
+           (nu : NtSet.t),
+      nullable_set_sound nu g
+      -> nullable_set_sound (nullablePass g.(prods) nu) g.
+  Proof.
+    intros g nu Hsou.
+    apply nullablePass_preserves_soundness' with (pre := []); auto.
+  Qed.
+  
+  Lemma mkNullableSet'_preserves_soundness :
+    forall (g  : grammar)
+           (nu : NtSet.t),
+      nullable_set_sound nu g
+      -> nullable_set_sound (mkNullableSet' g.(prods) nu) g.
+  Proof.
+    intros g nu.
+    remember (countNullableCandidates g.(prods) nu) as card.
+    generalize dependent nu.
+    induction card using lt_wf_ind.
+    intros nu Hcard Hsou; subst.
+    rewrite mkNullableSet'_eq_body; simpl.
+    destruct (NtSet.eq_dec nu (nullablePass g.(prods) nu)) as [Heq | Hneq]; auto.
+    eapply H; clear H; eauto.
+    - apply nullablePass_neq_candidates_lt; auto. 
+    - apply nullablePass_preserves_soundness; auto.
+  Qed.
+  
+  Lemma empty_nu_sound :
+    forall (g : grammar),
+      nullable_set_sound NtSet.empty g.
+  Proof.
+    unfold nullable_set_sound; ND.fsetdec.
+  Qed.
+  
+  Theorem mkNullableSet_sound :
+    forall (g : grammar),
+      nullable_set_sound (mkNullableSet g) g.
+  Proof.
+    intros g.
+    unfold mkNullableSet.
+    apply mkNullableSet'_preserves_soundness.
+    apply empty_nu_sound.
+  Qed.
+  
+  (* Completeness *)
+  
+  Lemma nullablePass_add_equal :
+    forall ps x nu,
+      NtSet.In x nu
+      -> NtSet.Equal (nullablePass ps nu) (NtSet.add x (nullablePass ps nu)).
+  Proof.
+    intros ps.
+    induction ps as [| (x', ys) ps]; intros x nu Hin; simpl in *.
+    - ND.fsetdec.
+    - destruct (nullableGamma ys (nullablePass ps nu)); auto.
+      apply IHps in Hin; ND.fsetdec.
+  Qed.
+  
+  Lemma nullable_gamma_nullableGamma_true :
+    forall g ys nu,
+      nullable_gamma g ys
+      -> (forall x, In (NT x) ys -> NtSet.In x nu)
+      -> nullableGamma ys nu = true.
+  Proof.
+    intros g.
+    induction ys as [| sym syms]; intros nu Hng Hall; auto.
+    destruct sym as [y | x].
+    - inv Hng.
+      inv H1. (* LEMMA *)
+    - simpl. 
+      assert (In (NT x) (NT x :: syms)) by (left; auto).
+      apply Hall in H.
+      rewrite <- NtSet.mem_spec in H.
+      rewrite H.
+      apply IHsyms.
+      + inv Hng; auto.
+      + firstorder.
+  Qed.
+  
+  Lemma nu_equal_nullableGamma_eq :
+    forall nu nu' gamma,
+      NtSet.Equal nu nu'
+      -> nullableGamma gamma nu = nullableGamma gamma nu'.
+  Proof.
+    intros nu nu' gamma.
+    induction gamma as [| sym syms]; intros Heq; simpl in *; auto.
+    destruct sym as [y | x]; auto.
+    destruct (NtSet.mem x nu) eqn:Hmem; destruct (NtSet.mem x nu') eqn:Hmem'; auto.
+    - rewrite NtSet.mem_spec in Hmem.
+      apply Heq in Hmem.
+      rewrite <- NtSet.mem_spec in Hmem; congruence.
+    - rewrite NtSet.mem_spec in Hmem'.
+      apply Heq in Hmem'.
+      rewrite <- NtSet.mem_spec in Hmem'; congruence.
+  Qed.
+  
+  Lemma nullablePass_right_in_left_in :
+    forall (g  : grammar)
+           (x  : nonterminal)
+           (ys : list symbol)
+           (suf pre : list production),
+      pre ++ suf = g.(prods)
+      -> In (x, ys) suf
+      -> nullable_gamma g ys
+      -> forall nu,
+          NtSet.Equal nu (nullablePass suf nu)
+          -> (forall x, In (NT x) ys -> NtSet.In x nu)
+          -> NtSet.In x nu.
+  Proof.
+    intros g x ys suf.
+    induction suf as [| (x', ys') suf]; intros pre Happ Hin Hng nu Heq Hall.
+    - inv Hin.
+    - destruct Hin.
+      + inv H; simpl in *.
+        destruct (nullableGamma ys (nullablePass suf nu)) eqn:Hf.
+        * ND.fsetdec.
+        * exfalso.
+          eapply nullable_gamma_nullableGamma_true in Hng; eauto.
+          erewrite nu_equal_nullableGamma_eq in Hng; eauto.
+          congruence.
+      + apply IHsuf with (pre := pre ++ [(x', ys')]); auto.
+        * rewrite <- app_assoc; auto. 
+        * simpl in *. 
+          destruct (nullableGamma ys' (nullablePass suf nu)).
+          -- assert (NtSet.In x' nu) by ND.fsetdec. 
+             apply nullablePass_add_equal with (ps := suf) in H0.
+             ND.fsetdec.
+          -- auto.
+  Qed.
+
+(* Slight rephrasing of nullable_set_complete so that it's 
+   compatible with induction on a nullable_sym judgment *)
+Definition nullable_set_complete' nu g :=
+  forall (sym : symbol)
+         (x   : nonterminal), 
+    nullable_sym g sym
+    -> sym = NT x
+    -> NtSet.In x nu.
+
+(* Proof that it's equivalent *)
+Lemma ns_complete'_complete :
+  forall g nu,
+    nullable_set_complete' nu g
+    <-> nullable_set_complete nu g.
+Proof.
+  split; intros.
+  - unfold nullable_set_complete; eauto.
+  - unfold nullable_set_complete'; intros; subst; auto.
+Qed.
+
+(* Proof that when the iteration in mkNullableSet' converges, 
+   the resulting  NULLABLE set is complete *)
+Lemma nullablePass_equal_complete' :
+  forall g nu,
+    NtSet.Equal nu (nullablePass g.(prods) nu)
+    -> nullable_set_complete' nu g.
+Proof.
+  intros g nu Heq.
+  unfold nullable_set_complete'.
+  intros sym x Hns.
+  revert x.
+  induction Hns using nullable_sym_mutual_ind with
+      (P  := fun sym (pf : nullable_sym g sym) =>
+               forall x, sym = NT x -> NtSet.In x nu)
+      (P0 := fun gamma (pf : nullable_gamma g gamma) =>
+               forall x, In (NT x) gamma -> NtSet.In x nu).
+  - intros x' Heq'.
+    inv Heq'.
+    eapply nullablePass_right_in_left_in with 
+    (pre := nil); simpl; eauto.
+  - intros x Hin.
+    inv Hin.
+  - intros x Hin.
+    destruct Hin.
+    + subst.
+      apply IHHns; auto.
+    + auto.
+Qed.
+
+Lemma nullablePass_equal_complete :
+  forall g nu,
+    NtSet.Equal nu (nullablePass g.(prods) nu)
+    -> nullable_set_complete nu g.
+Proof.
+  intros.
+  apply ns_complete'_complete.
+  apply nullablePass_equal_complete'; auto.
+Qed.
+
+Lemma mkNullableSet'_complete :
+  forall g nu,
+    nullable_set_complete (mkNullableSet' g.(prods) nu) g.
+Proof.
+  intros g nu.
+  remember (countNullableCandidates g.(prods) nu) as card.
+  generalize dependent nu.
+  induction card using lt_wf_ind.
+  intros nu Hcard; subst.
+  rewrite mkNullableSet'_eq_body; simpl.
+  destruct (NtSet.eq_dec nu (nullablePass g.(prods) nu)) as [Heq | Hneq].
+  - apply nullablePass_equal_complete; auto.
+  - eapply H; clear H; eauto.
+    apply nullablePass_neq_candidates_lt; auto.
+Qed.
+
+Theorem mkNullableSet_complete :
+  forall g,
+    nullable_set_complete (mkNullableSet g) g.
+Proof.
+  intros g.
+  unfold mkNullableSet.
+  apply mkNullableSet'_complete.
+Qed.
+
+(* Putting both mkNullableSet correctness properties into a single theorem *)
+
+Theorem mkNullableSet_correct :
+  forall (g : grammar),
+    nullable_set_for (mkNullableSet g) g.
+Proof.
+  intros g.
+  unfold nullable_set_for; split.
+  - apply mkNullableSet_sound.
+  - apply mkNullableSet_complete.
+Qed.
+
+End NullableProofsFn.
