Utils.v
@@ -1,7 +1,0 @@
-Require Import List.
-Require Import Grammar.
-
-Module UtilsFn (Export G : GRAMMAR).
-
-
-End UtilsFn.
